

Formal Deduction

Proving arguments in a purely syntactic way using formal rules for deduction. The goal is to define a relation called formal deducibility (\vdash) to mechanically/syntactically check the truth of a proof. These proofs will not rely on any semantic properties which is the main distinction

The Main Idea

Formal Deducibility is a relation between a set of formulas Σ (premises) and formula A (conclusion).

This is written as: $\Sigma \vdash A \rightarrow A$ is formally deducible (provable) from Σ

$\Sigma \cup A = \Sigma, A$
 $\Sigma \cup \Sigma' = \Sigma, \Sigma'$ } common rewrites

The 11 Rules of Formal Deduction

1. $A \vdash A \rightarrow$ Reflexivity

2. if: $\Sigma \vdash A$
then: $\Sigma, \Sigma' \vdash A \rightarrow$ Addition of premises (+)

3. if: $\Sigma, \neg A \vdash B$
and: $\Sigma, \neg A \vdash \neg B \rightarrow$ \neg elimination
then: $\Sigma \vdash A$

4. if: $\Sigma \vdash A \rightarrow B$
and: $\Sigma \vdash A \rightarrow$ \rightarrow elimination
then: $\Sigma \vdash B$

5. if: $\Sigma, A \vdash B$
then: $\Sigma \vdash A \rightarrow B \rightarrow$ \rightarrow introduction

6. if: $\Sigma \vdash A \wedge B$
then: $\Sigma \vdash A \rightarrow$ \wedge elimination
and: $\Sigma \vdash B$

7. if: $\Sigma \vdash A$
and: $\Sigma \vdash B \rightarrow$ \wedge introduction
then: $\Sigma \vdash A \wedge B$

8. if: $\Sigma, A \vdash C$
and: $\Sigma, B \vdash C \rightarrow$ \vee elimination
then: $\Sigma, A \vee B \vdash C$

9. if: $\Sigma \vdash A$
then: $\Sigma \vdash A \vee B \rightarrow$ \vee introduction
and: $\Sigma \vdash B \vee A$

10. if: $\Sigma \vdash A \leftrightarrow B$
and: $\Sigma \vdash A \rightarrow$ \leftrightarrow elimination
then: $\Sigma \vdash B$

11. if: $\Sigma, A \vdash B$
and: $\Sigma, B \vdash A \rightarrow$ \leftrightarrow introduction
then: $\Sigma \vdash A \leftrightarrow B$

Each of these deductibility formulas can be formally expressed as "is a theorem" like $\Sigma \vdash A$ is a theorem, basically meaning A is provable by the premises of Σ . The meaning of theorem is that this statement can be proved valid by this logic system

\vdash vs \models :

The distinction between deductibility and tautological equivalence is crucial

$\Sigma \vdash A$: A is provable from Σ

$\Sigma \models A$: A is true in all models Σ is true (equivalent)

Example 1:

(ϵ) if $A \in \Sigma$ (membership rule) \rightarrow if A is a premise
then $\Sigma \vdash A$ A can be derived from Σ

Proof: Suppose $A \in \Sigma$ and $\Sigma' = \Sigma - \{A\}$ (Σ is $A \cup \Sigma'$)

1) $A \vdash A$ (by ref) \rightarrow generated by reflexivity, $A \vdash A$ is always a valid starting point

2) $A, \Sigma' \vdash A$ (by +, (1)) \rightarrow generated by + rule applied to step 1.

These steps constitute a formal proof of $\Sigma \vdash A$. (ϵ) is now formally proven and is a new theorem. This proof is basically saying if $A \vdash A$ and $A \in \Sigma$, then $\Sigma \vdash A$ by breaking Σ into Σ' and A .

Proving Hypothetical Syllogism with Formal Deduction

(E) $A \rightarrow B, B \rightarrow C \vdash A \rightarrow C$

(1) $A \rightarrow B, B \rightarrow C, A \vdash A \rightarrow B$ (by (E)) \rightarrow from premises

(2) $A \rightarrow B, B \rightarrow C, A \vdash A$ (by (E)) \rightarrow from premises

(3) $A \rightarrow B, B \rightarrow C, A \vdash B$ (by (\rightarrow elim), (1), (2)) $\rightarrow A \rightarrow B$ and $A \therefore B$

(4) $A \rightarrow B, B \rightarrow C, B \vdash C$ (by (E))

(5) $A \rightarrow B, B \rightarrow C, A \vdash C$ (by (\rightarrow elim), (3), (4)) $\rightarrow B \rightarrow C$ and $B \therefore C$

(6) $A \rightarrow B, B \rightarrow C \vdash A \rightarrow C$ (by (\rightarrow intro), from (5) discharging A) $\rightarrow A$ and $C \therefore A \rightarrow C$

\hookrightarrow This discharges the temporary assumption that A is true.